new/golang/defn.v
@@ -1,3 +1,2 @@
 From New.golang.defn Require Export core.
-From New.golang.defn Require Export
-  slice string defer chan.
+From New.golang.defn Require Export slice string defer chan.
