new/golang/defn/core.v
@@ -1,4 +1,3 @@
 (* a set of "core" libraries for goose code, intended to bootstrap models that
-are written in Go and translated with goose *)
-From Perennial.goose_lang Require Export lang.
-From New.golang.defn Require Export exception pkg loop.
+   are written in Go and translated with goose *)
+From New.golang.defn Require Export exception pkg loop slice map predeclared.
