new/trusted_code/github_com/goose_lang/primitive.v
@@ -1,4 +1,3 @@
-From New.code Require Import sync.
 From New.golang.defn Require Import core slice lock.
 
 Module primitive.
@@ -26,40 +25,40 @@ this in GooseLang, so we just loop. *)
   Definition UInt64Putⁱᵐᵖˡ : val :=
     λ: "p" "n",
       exception_do (
-      do: (slice.elem_ref #uint8T "p" #(W64 0)) <-[#uint8T] to_u8 ("n" ≫ #(W64 (0*8)));;;
-      do: (slice.elem_ref #uint8T "p" #(W64 1)) <-[#uint8T] to_u8 ("n" ≫ #(W64 (1*8)));;;
-      do: (slice.elem_ref #uint8T "p" #(W64 2)) <-[#uint8T] to_u8 ("n" ≫ #(W64 (2*8)));;;
-      do: (slice.elem_ref #uint8T "p" #(W64 3)) <-[#uint8T] to_u8 ("n" ≫ #(W64 (3*8)));;;
-      do: (slice.elem_ref #uint8T "p" #(W64 4)) <-[#uint8T] to_u8 ("n" ≫ #(W64 (4*8)));;;
-      do: (slice.elem_ref #uint8T "p" #(W64 5)) <-[#uint8T] to_u8 ("n" ≫ #(W64 (5*8)));;;
-      do: (slice.elem_ref #uint8T "p" #(W64 6)) <-[#uint8T] to_u8 ("n" ≫ #(W64 (6*8)));;;
-      do: (slice.elem_ref #uint8T "p" #(W64 7)) <-[#uint8T] to_u8 ("n" ≫ #(W64 (7*8)))).
+      do: (IndexRef (go.SliceType go.uint8) "p" #(W64 0)) <-[go.uint8] to_u8 ("n" ≫ #(W64 (0*8)));;;
+      do: (IndexRef (go.SliceType go.uint8) "p" #(W64 1)) <-[go.uint8] to_u8 ("n" ≫ #(W64 (1*8)));;;
+      do: (IndexRef (go.SliceType go.uint8) "p" #(W64 2)) <-[go.uint8] to_u8 ("n" ≫ #(W64 (2*8)));;;
+      do: (IndexRef (go.SliceType go.uint8) "p" #(W64 3)) <-[go.uint8] to_u8 ("n" ≫ #(W64 (3*8)));;;
+      do: (IndexRef (go.SliceType go.uint8) "p" #(W64 4)) <-[go.uint8] to_u8 ("n" ≫ #(W64 (4*8)));;;
+      do: (IndexRef (go.SliceType go.uint8) "p" #(W64 5)) <-[go.uint8] to_u8 ("n" ≫ #(W64 (5*8)));;;
+      do: (IndexRef (go.SliceType go.uint8) "p" #(W64 6)) <-[go.uint8] to_u8 ("n" ≫ #(W64 (6*8)));;;
+      do: (IndexRef (go.SliceType go.uint8) "p" #(W64 7)) <-[go.uint8] to_u8 ("n" ≫ #(W64 (7*8)))).
 
   Definition UInt64Getⁱᵐᵖˡ : val := λ: "p",
-      let: "v0" := to_u64 ![#uint8T](slice.elem_ref #uint8T "p" #(W64 0)) in
-      let: "v1" := to_u64 ![#uint8T](slice.elem_ref #uint8T "p" #(W64 1)) in
-      let: "v2" := to_u64 ![#uint8T](slice.elem_ref #uint8T "p" #(W64 2)) in
-      let: "v3" := to_u64 ![#uint8T](slice.elem_ref #uint8T "p" #(W64 3)) in
-      let: "v4" := to_u64 ![#uint8T](slice.elem_ref #uint8T "p" #(W64 4)) in
-      let: "v5" := to_u64 ![#uint8T](slice.elem_ref #uint8T "p" #(W64 5)) in
-      let: "v6" := to_u64 ![#uint8T](slice.elem_ref #uint8T "p" #(W64 6)) in
-      let: "v7" := to_u64 ![#uint8T](slice.elem_ref #uint8T "p" #(W64 7)) in
+      let: "v0" := to_u64 ![go.uint8](IndexRef (go.SliceType go.uint8) "p" #(W64 0)) in
+      let: "v1" := to_u64 ![go.uint8](IndexRef (go.SliceType go.uint8) "p" #(W64 1)) in
+      let: "v2" := to_u64 ![go.uint8](IndexRef (go.SliceType go.uint8) "p" #(W64 2)) in
+      let: "v3" := to_u64 ![go.uint8](IndexRef (go.SliceType go.uint8) "p" #(W64 3)) in
+      let: "v4" := to_u64 ![go.uint8](IndexRef (go.SliceType go.uint8) "p" #(W64 4)) in
+      let: "v5" := to_u64 ![go.uint8](IndexRef (go.SliceType go.uint8) "p" #(W64 5)) in
+      let: "v6" := to_u64 ![go.uint8](IndexRef (go.SliceType go.uint8) "p" #(W64 6)) in
+      let: "v7" := to_u64 ![go.uint8](IndexRef (go.SliceType go.uint8) "p" #(W64 7)) in
       "v0" `or` ("v1" `or` ("v2" `or` ("v3" `or` ("v4" `or` ("v5" `or` ("v6" `or` "v7"
           ≪ #(W64 8)) ≪ #(W64 8)) ≪ #(W64 8)) ≪ #(W64 8)) ≪ #(W64 8)) ≪ #(W64 8)) ≪ #(W64 8).
 
   Definition UInt32Putⁱᵐᵖˡ : val :=
     λ: "p" "n",
       exception_do (
-      do: (slice.elem_ref #uint8T "p" #(W64 0)) <-[#uint8T] to_u8 ("n" ≫ #(W32 (0*8)));;;
-      do: (slice.elem_ref #uint8T "p" #(W64 1)) <-[#uint8T] to_u8 ("n" ≫ #(W32 (1*8)));;;
-      do: (slice.elem_ref #uint8T "p" #(W64 2)) <-[#uint8T] to_u8 ("n" ≫ #(W32 (2*8)));;;
-      do: (slice.elem_ref #uint8T "p" #(W64 3)) <-[#uint8T] to_u8 ("n" ≫ #(W32 (3*8)))).
+      do: (IndexRef (go.SliceType go.uint8) "p" #(W64 0)) <-[go.uint8] to_u8 ("n" ≫ #(W32 (0*8)));;;
+      do: (IndexRef (go.SliceType go.uint8) "p" #(W64 1)) <-[go.uint8] to_u8 ("n" ≫ #(W32 (1*8)));;;
+      do: (IndexRef (go.SliceType go.uint8) "p" #(W64 2)) <-[go.uint8] to_u8 ("n" ≫ #(W32 (2*8)));;;
+      do: (IndexRef (go.SliceType go.uint8) "p" #(W64 3)) <-[go.uint8] to_u8 ("n" ≫ #(W32 (3*8)))).
 
   Definition UInt32Getⁱᵐᵖˡ : val := λ: "p",
-      let: "v0" := to_u32 ![#uint8T](slice.elem_ref #uint8T "p" #(W64 0)) in
-      let: "v1" := to_u32 ![#uint8T](slice.elem_ref #uint8T "p" #(W64 1)) in
-      let: "v2" := to_u32 ![#uint8T](slice.elem_ref #uint8T "p" #(W64 2)) in
-      let: "v3" := to_u32 ![#uint8T](slice.elem_ref #uint8T "p" #(W64 3)) in
+      let: "v0" := to_u32 ![go.uint8](IndexRef (go.SliceType go.uint8) "p" #(W64 0)) in
+      let: "v1" := to_u32 ![go.uint8](IndexRef (go.SliceType go.uint8) "p" #(W64 1)) in
+      let: "v2" := to_u32 ![go.uint8](IndexRef (go.SliceType go.uint8) "p" #(W64 2)) in
+      let: "v3" := to_u32 ![go.uint8](IndexRef (go.SliceType go.uint8) "p" #(W64 3)) in
       "v0" `or` ("v1" `or` ("v2" `or` ("v3" ≪ #(W32 8)) ≪ #(W32 8)) ≪ #(W32 8)) ≪ #(W32 8).
 
   Definition Millisecond: val := #(W64 1000000).
@@ -70,9 +69,6 @@ this in GooseLang, so we just loop. *)
   Definition TimeNowⁱᵐᵖˡ : val := λ: <>, ArbitraryInt.
 
   Definition AfterFuncⁱᵐᵖˡ : val := λ: "duration" "f", Fork "f" ;; ref "f".
-
-  Definition WaitTimeoutⁱᵐᵖˡ : val := λ: "l" "timeout",
-      method_call #sync #"Cond" "Wait" "l".
 
   Definition RandomUint64ⁱᵐᵖˡ : val := λ: <>, ArbitraryInt.
 
@@ -85,7 +81,7 @@ this in GooseLang, so we just loop. *)
   Definition AssumeNoStringOverflowⁱᵐᵖˡ : val :=
     λ: "s", assume.assume (IsNoStringOverflow "s").
 
-  Definition Mutex := boolT.
+  Definition Mutexⁱᵐᵖˡ := go.bool.
 
   Definition Mutex__Lockⁱᵐᵖˡ : val :=
     λ: "m" <>, lock.lock "m".
